floyd/Funspec_old_Notation.v
@@ -1,6 +1,4 @@
-Require Import VST.floyd.funspec_old.
+Require Export VST.floyd.funspec_old.
 
 Global Close Scope funspec_scope.
 Global Open Scope old_funspec_scope.
-
-Notation "'main_pre'" := (old_main_pre) : old_funspec_scope.
