progs/conc_queue_specs.v
@@ -6,7 +6,7 @@ Require Import VST.floyd.library.
 
 Set Bullet Behavior "Strict Subproofs".
 
-Global Open Scope old_funspec_scope.
+Require Export VST.floyd.Funspec_old_Notation.
 Instance CompSpecs : compspecs. make_compspecs prog. Defined.
 Definition Vprog : varspecs. mk_varspecs prog. Defined.
 
