progs/conclib.v
@@ -6,6 +6,7 @@ Require Export VST.floyd.proofauto.
 Require Import VST.floyd.library.
 Require Export VST.floyd.sublist.
 Import LiftNotation.
+(*Require Export VST.floyd.Funspec_old_Notation.*)
 
 (* general list lemmas *)
 Notation vint z := (Vint (Int.repr z)).
@@ -3146,7 +3147,7 @@ Ltac start_dep_function :=
 
 (* Notations for dependent funspecs *)
 Notation "'TYPE' A 'WITH'  x1 : t1 , x2 : t2 'PRE'  [ u , .. , v ] P 'POST' [ tz ] Q" :=
-     (mk_funspec ((cons u%formals .. (cons v%formals nil) ..), tz) cc_default A
+     (mk_funspec ((cons u%type .. (cons v%type nil) ..), tz) cc_default A
   (fun (ts: list Type) (x: t1*t2) =>
      match x with (x1,x2) => P%assert end)
   (fun (ts: list Type) (x: t1*t2) =>
@@ -3155,7 +3156,7 @@ Notation "'TYPE' A 'WITH'  x1 : t1 , x2 : t2 'PRE'  [ u , .. , v ] P 'POST' [ tz
              P at level 100, Q at level 100).
 
 Notation "'TYPE' A 'WITH'  x1 : t1 , x2 : t2 , x3 : t3 'PRE'  [ u , .. , v ] P 'POST' [ tz ] Q" :=
-     (mk_funspec ((cons u%formals .. (cons v%formals nil) ..), tz) cc_default A
+     (mk_funspec ((cons u%type .. (cons v%type nil) ..), tz) cc_default A
   (fun (ts: list Type) (x: t1*t2*t3) =>
      match x with (x1,x2,x3) => P%assert end)
   (fun (ts: list Type) (x: t1*t2*t3) =>
@@ -3164,7 +3165,7 @@ Notation "'TYPE' A 'WITH'  x1 : t1 , x2 : t2 , x3 : t3 'PRE'  [ u , .. , v ] P '
              P at level 100, Q at level 100).
 
 Notation "'TYPE' A 'WITH'  x1 : t1 , x2 : t2 , x3 : t3 , x4 : t4 'PRE'  [ u , .. , v ] P 'POST' [ tz ] Q" :=
-     (mk_funspec ((cons u%formals .. (cons v%formals nil) ..), tz) cc_default A
+     (mk_funspec ((cons u%type .. (cons v%type nil) ..), tz) cc_default A
   (fun (ts: list Type) (x: t1*t2*t3*t4) =>
      match x with (x1,x2,x3,x4) => P%assert end)
   (fun (ts: list Type) (x: t1*t2*t3*t4) =>
@@ -3173,7 +3174,7 @@ Notation "'TYPE' A 'WITH'  x1 : t1 , x2 : t2 , x3 : t3 , x4 : t4 'PRE'  [ u , ..
              P at level 100, Q at level 100).
 
 Notation "'TYPE' A 'WITH'  x1 : t1 , x2 : t2 , x3 : t3 , x4 : t4 , x5 : t5 'PRE'  [ u , .. , v ] P 'POST' [ tz ] Q" :=
-     (mk_funspec ((cons u%formals .. (cons v%formals nil) ..), tz) cc_default A
+     (mk_funspec ((cons u%type .. (cons v%type nil) ..), tz) cc_default A
   (fun (ts: list Type) (x: t1*t2*t3*t4*t5) =>
      match x with (x1,x2,x3,x4,x5) => P%assert end)
   (fun (ts: list Type) (x: t1*t2*t3*t4*t5) =>
@@ -3183,7 +3184,7 @@ Notation "'TYPE' A 'WITH'  x1 : t1 , x2 : t2 , x3 : t3 , x4 : t4 , x5 : t5 'PRE'
              P at level 100, Q at level 100).
 
 Notation "'TYPE' A 'WITH'  x1 : t1 , x2 : t2 , x3 : t3 , x4 : t4 , x5 : t5 , x6 : t6 'PRE'  [ u , .. , v ] P 'POST' [ tz ] Q" :=
-     (mk_funspec ((cons u%formals .. (cons v%formals nil) ..), tz) cc_default A
+     (mk_funspec ((cons u%type .. (cons v%type nil) ..), tz) cc_default A
   (fun (ts: list Type) (x: t1*t2*t3*t4*t5*t6) =>
      match x with (x1,x2,x3,x4,x5,x6) => P%assert end)
   (fun (ts: list Type) (x: t1*t2*t3*t4*t5*t6) =>
@@ -3193,7 +3194,7 @@ Notation "'TYPE' A 'WITH'  x1 : t1 , x2 : t2 , x3 : t3 , x4 : t4 , x5 : t5 , x6 
              P at level 100, Q at level 100).
 
 Notation "'TYPE' A 'WITH'  x1 : t1 , x2 : t2 , x3 : t3 , x4 : t4 , x5 : t5 , x6 : t6 , x7 : t7 'PRE'  [ u , .. , v ] P 'POST' [ tz ] Q" :=
-     (mk_funspec ((cons u%formals .. (cons v%formals nil) ..), tz) cc_default A
+     (mk_funspec ((cons u%type .. (cons v%type nil) ..), tz) cc_default A
   (fun (ts: list Type) (x: t1*t2*t3*t4*t5*t6*t7) =>
      match x with (x1,x2,x3,x4,x5,x6,x7) => P%assert end)
   (fun (ts: list Type) (x: t1*t2*t3*t4*t5*t6*t7) =>
@@ -3203,7 +3204,7 @@ Notation "'TYPE' A 'WITH'  x1 : t1 , x2 : t2 , x3 : t3 , x4 : t4 , x5 : t5 , x6 
              P at level 100, Q at level 100).
 
 Notation "'TYPE' A 'WITH'  x1 : t1 , x2 : t2 , x3 : t3 , x4 : t4 , x5 : t5 , x6 : t6 , x7 : t7 , x8 : t8 'PRE'  [ u , .. , v ] P 'POST' [ tz ] Q" :=
-     (mk_funspec ((cons u%formals .. (cons v%formals nil) ..), tz) cc_default A
+     (mk_funspec ((cons u%type .. (cons v%type nil) ..), tz) cc_default A
   (fun (ts: list Type) (x: t1*t2*t3*t4*t5*t6*t7*t8) =>
      match x with (x1,x2,x3,x4,x5,x6,x7,x8) => P%assert end)
   (fun (ts: list Type) (x: t1*t2*t3*t4*t5*t6*t7*t8) =>
@@ -3213,7 +3214,7 @@ Notation "'TYPE' A 'WITH'  x1 : t1 , x2 : t2 , x3 : t3 , x4 : t4 , x5 : t5 , x6 
              P at level 100, Q at level 100).
 
 Notation "'TYPE' A 'WITH'  x1 : t1 , x2 : t2 , x3 : t3 , x4 : t4 , x5 : t5 , x6 : t6 , x7 : t7 , x8 : t8 , x9 : t9 'PRE'  [ u , .. , v ] P 'POST' [ tz ] Q" :=
-     (mk_funspec ((cons u%formals .. (cons v%formals nil) ..), tz) cc_default A
+     (mk_funspec ((cons u%type .. (cons v%type nil) ..), tz) cc_default A
   (fun (ts: list Type) (x: t1*t2*t3*t4*t5*t6*t7*t8*t9) =>
      match x with (x1,x2,x3,x4,x5,x6,x7,x8,x9) => P%assert end)
   (fun (ts: list Type) (x: t1*t2*t3*t4*t5*t6*t7*t8*t9) =>
@@ -3223,7 +3224,7 @@ Notation "'TYPE' A 'WITH'  x1 : t1 , x2 : t2 , x3 : t3 , x4 : t4 , x5 : t5 , x6 
              P at level 100, Q at level 100).
 
 Notation "'TYPE' A 'WITH'  x1 : t1 , x2 : t2 , x3 : t3 , x4 : t4 , x5 : t5 , x6 : t6 , x7 : t7 , x8 : t8 , x9 : t9 , x10 : t10 'PRE'  [ u , .. , v ] P 'POST' [ tz ] Q" :=
-     (mk_funspec ((cons u%formals .. (cons v%formals nil) ..), tz) cc_default A
+     (mk_funspec ((cons u%type .. (cons v%type nil) ..), tz) cc_default A
   (fun (ts: list Type) (x: t1*t2*t3*t4*t5*t6*t7*t8*t9*t10) =>
      match x with (x1,x2,x3,x4,x5,x6,x7,x8,x9,x10) => P%assert end)
   (fun (ts: list Type) (x: t1*t2*t3*t4*t5*t6*t7*t8*t9*t10) =>
@@ -3233,7 +3234,7 @@ Notation "'TYPE' A 'WITH'  x1 : t1 , x2 : t2 , x3 : t3 , x4 : t4 , x5 : t5 , x6 
              P at level 100, Q at level 100).
 
 Notation "'TYPE' A 'WITH'  x1 : t1 , x2 : t2 , x3 : t3 , x4 : t4 , x5 : t5 , x6 : t6 , x7 : t7 , x8 : t8 , x9 : t9 , x10 : t10 'PRE'  [ u , .. , v ] P 'POST' [ tz ] Q" :=
-     (mk_funspec ((cons u%formals .. (cons v%formals nil) ..), tz) cc_default A
+     (mk_funspec ((cons u%type .. (cons v%type nil) ..), tz) cc_default A
   (fun (ts: list Type) (x: t1*t2*t3*t4*t5*t6*t7*t8*t9*t10) =>
      match x with (x1,x2,x3,x4,x5,x6,x7,x8,x9,x10) => P%assert end)
   (fun (ts: list Type) (x: t1*t2*t3*t4*t5*t6*t7*t8*t9*t10) =>
@@ -3243,7 +3244,7 @@ Notation "'TYPE' A 'WITH'  x1 : t1 , x2 : t2 , x3 : t3 , x4 : t4 , x5 : t5 , x6 
              P at level 100, Q at level 100).
 
 Notation "'TYPE' A 'WITH'  x1 : t1 , x2 : t2 , x3 : t3 , x4 : t4 , x5 : t5 , x6 : t6 , x7 : t7 , x8 : t8 , x9 : t9 , x10 : t10 , x11 : t11 'PRE'  [ u , .. , v ] P 'POST' [ tz ] Q" :=
-     (mk_funspec ((cons u%formals .. (cons v%formals nil) ..), tz) cc_default A
+     (mk_funspec ((cons u%type .. (cons v%type nil) ..), tz) cc_default A
   (fun (ts: list Type) (x: t1*t2*t3*t4*t5*t6*t7*t8*t9*t10*t11) =>
      match x with (x1,x2,x3,x4,x5,x6,x7,x8,x9,x10,x11) => P%assert end)
   (fun (ts: list Type) (x: t1*t2*t3*t4*t5*t6*t7*t8*t9*t10*t11) =>
@@ -3254,7 +3255,7 @@ Notation "'TYPE' A 'WITH'  x1 : t1 , x2 : t2 , x3 : t3 , x4 : t4 , x5 : t5 , x6 
              P at level 100, Q at level 100).
 
 Notation "'TYPE' A 'WITH'  x1 : t1 , x2 : t2 , x3 : t3 , x4 : t4 , x5 : t5 , x6 : t6 , x7 : t7 , x8 : t8 , x9 : t9 , x10 : t10 , x11 : t11 , x12 : t12 'PRE'  [ u , .. , v ] P 'POST' [ tz ] Q" :=
-     (mk_funspec ((cons u%formals .. (cons v%formals nil) ..), tz) cc_default A
+     (mk_funspec ((cons u%type .. (cons v%type nil) ..), tz) cc_default A
   (fun (ts: list Type) (x: t1*t2*t3*t4*t5*t6*t7*t8*t9*t10*t11*t12) =>
      match x with (x1,x2,x3,x4,x5,x6,x7,x8,x9,x10,x11,x12) => P%assert end)
   (fun (ts: list Type) (x: t1*t2*t3*t4*t5*t6*t7*t8*t9*t10*t11*t12) =>
@@ -3265,7 +3266,7 @@ Notation "'TYPE' A 'WITH'  x1 : t1 , x2 : t2 , x3 : t3 , x4 : t4 , x5 : t5 , x6 
              P at level 100, Q at level 100).
 
 Notation "'TYPE' A 'WITH'  x1 : t1 , x2 : t2 , x3 : t3 , x4 : t4 , x5 : t5 , x6 : t6 , x7 : t7 , x8 : t8 , x9 : t9 , x10 : t10 , x11 : t11 , x12 : t12 , x13 : t13 'PRE'  [ u , .. , v ] P 'POST' [ tz ] Q" :=
-     (mk_funspec ((cons u%formals .. (cons v%formals nil) ..), tz) cc_default A
+     (mk_funspec ((cons u%type .. (cons v%type nil) ..), tz) cc_default A
   (fun (ts: list Type) (x: t1*t2*t3*t4*t5*t6*t7*t8*t9*t10*t11*t12*t13) =>
      match x with (x1,x2,x3,x4,x5,x6,x7,x8,x9,x10,x11,x12,x13) => P%assert end)
   (fun (ts: list Type) (x: t1*t2*t3*t4*t5*t6*t7*t8*t9*t10*t11*t12*t13) =>
@@ -3276,7 +3277,7 @@ Notation "'TYPE' A 'WITH'  x1 : t1 , x2 : t2 , x3 : t3 , x4 : t4 , x5 : t5 , x6 
              P at level 100, Q at level 100).
 
 Notation "'TYPE' A 'WITH'  x1 : t1 , x2 : t2 , x3 : t3 , x4 : t4 , x5 : t5 , x6 : t6 , x7 : t7 , x8 : t8 , x9 : t9 , x10 : t10 , x11 : t11 , x12 : t12 , x13 : t13 , x14 : t14 'PRE'  [ u , .. , v ] P 'POST' [ tz ] Q" :=
-     (mk_funspec ((cons u%formals .. (cons v%formals nil) ..), tz) cc_default A
+     (mk_funspec ((cons u%type .. (cons v%type nil) ..), tz) cc_default A
   (fun (ts: list Type) (x: t1*t2*t3*t4*t5*t6*t7*t8*t9*t10*t11*t12*t13*t14) =>
      match x with (x1,x2,x3,x4,x5,x6,x7,x8,x9,x10,x11,x12,x13,x14) => P%assert end)
   (fun (ts: list Type) (x: t1*t2*t3*t4*t5*t6*t7*t8*t9*t10*t11*t12*t13*t14) =>
