progs/tutorial1.v
@@ -1,6 +1,6 @@
 Require Import VST.floyd.proofauto.
 Require Import VST.progs.sumarray.
-Global Open Scope old_funspec_scope.
+Require Export VST.floyd.Funspec_old_Notation.
 Instance CompSpecs : compspecs. make_compspecs prog. Defined.
 Definition Vprog : varspecs.  mk_varspecs prog. Defined.
 Definition Gprog: funspecs := nil.
