progs/verif_append.v
@@ -4,7 +4,7 @@ Require Import VST.progs.append.
 
 Open Scope logic.
 
-Global Open Scope old_funspec_scope.
+Require Export VST.floyd.Funspec_old_Notation.
 Instance CompSpecs : compspecs. make_compspecs prog. Defined.
 Definition Vprog : varspecs. mk_varspecs prog. Defined.
 Instance LS: listspec _list _tail (fun _ _ => emp).
