progs/verif_fib.v
@@ -1,6 +1,6 @@
 Require Import VST.floyd.proofauto.
 Require Import VST.progs.fib.
-Global Open Scope old_funspec_scope.
+Require Export VST.floyd.Funspec_old_Notation.
 Instance CompSpecs : compspecs. make_compspecs prog. Defined.
 Definition Vprog : varspecs. mk_varspecs prog. Defined.
 
