progs/verif_incrN.v
@@ -2,7 +2,7 @@ Require Import VST.progs.conclib.
 Require Import VST.progs.ghosts.
 Require Import VST.progs.incrN.
 
-Global Open Scope old_funspec_scope.
+Require Export VST.floyd.Funspec_old_Notation.
 Instance CompSpecs : compspecs. make_compspecs prog. Defined.
 Definition Vprog : varspecs. mk_varspecs prog. Defined.
 
