progs/verif_loop_minus1.v
@@ -1,7 +1,7 @@
 Require Import VST.floyd.proofauto.
 Require Import VST.progs.loop_minus1.
 
-Global Open Scope old_funspec_scope.
+Require Export VST.floyd.Funspec_old_Notation.
 Instance CompSpecs : compspecs. make_compspecs prog. Defined.
 Definition Vprog : varspecs.  mk_varspecs prog. Defined.
 
