progs/verif_malloc.v
@@ -4,7 +4,7 @@ Require Import VST.floyd.library.
 (* First draft specs.  Not specifying that chunks are aligned. *)
 
 Require Import VST.progs.malloc.
-Global Open Scope old_funspec_scope.
+Require Export VST.floyd.Funspec_old_Notation.
 Instance CompSpecs : compspecs. make_compspecs prog. Defined.
 Definition Vprog : varspecs. mk_varspecs prog. Defined.
 Local Open Scope Z.
